#$\mathrm{binomial\ inversion}$

$$
f_n=\sum_{i=0}^n(-1)^i \binom{n}{i}g_i\Leftrightarrow g_i=\sum_{i=0}^n(-1)^{i} \binom{n}{i}f_i\\
$$

$\mathrm{another\ form:}$

​	$\mathrm{let}\ t_i=g_i\cdot(-1)^i$
$$
f_n=\sum_{i=0}^n\binom{n}{i}t_i\Leftrightarrow t_n=\sum_{i=0}^n(-1)^{n-i}\binom{n}{i}f_i\\
$$
$\mathrm{proof\ 1:}$

​	$\mathrm{there\ is\ a\ set\ S,\ and\ n\ subsets\ A_n,\ according\ to\ inclusion\ exclusion\ principle:}$
$$
|\bigcap_{n\ subsets}\overline{A_i}|=|S|+\sum_{i=1}^n (-1)^i|\bigcap_{i\ subsets}A_j|
$$
$\mathrm{suppose\ in\ a\ special\ case,\ which\ any\ m\ subsets\ have\ }$

​	$\mathrm{let}\ g_i=$
$$

$$
